Move modality record and instances to a separate file.

theories/proofmode/classes.v
@@ -1,4 +1,5 @@
 From iris.bi Require Export bi.
+From iris.proofmode Require Export modalities.
 From stdpp Require Import namespaces.
 Set Default Proof Using "Type".
 Import bi.
@@ -83,172 +84,22 @@ Arguments IntoPersistent {_} _ _%I _%I : simpl never.
 Arguments into_persistent {_} _ _%I _%I {_}.
 Hint Mode IntoPersistent + + ! - : typeclass_instances.
 
-(* The `iModIntro` tactic is not tied the Iris modalities, but can be
-instantiated with a variety of modalities.
-
-In order to plug in a modality, one has to decide for both the persistent and
-spatial what action should be performed upon introducing the modality:
-
-- Introduction is only allowed when the context is empty.
-- Introduction is only allowed when all hypotheses satisfy some predicate
-  `C : PROP → Prop` (where `C` should be a type class).
-- Introduction will transform each hypotheses using a type class
-  `C : PROP → PROP → Prop`, where the first parameter is the input and the
-  second parameter is the output. Hypotheses that cannot be transformed (i.e.
-  for which no instance of `C` can be found) will be cleared.
-- Introduction will clear the context.
-- Introduction will keep the context as-if.
-
-Formally, these actions correspond to the following inductive type: *)
-
-Inductive modality_intro_spec (PROP1 : bi) : bi → Type :=
-  | MIEnvIsEmpty {PROP2 : bi} : modality_intro_spec PROP1 PROP2
-  | MIEnvForall (C : PROP1 → Prop) : modality_intro_spec PROP1 PROP1
-  | MIEnvTransform {PROP2 : bi} (C : PROP2 → PROP1 → Prop) : modality_intro_spec PROP1 PROP2
-  | MIEnvClear {PROP2} : modality_intro_spec PROP1 PROP2
-  | MIEnvId : modality_intro_spec PROP1 PROP1.
-Arguments MIEnvIsEmpty {_ _}.
-Arguments MIEnvForall {_} _.
-Arguments MIEnvTransform {_ _} _.
-Arguments MIEnvClear {_ _}.
-Arguments MIEnvId {_}.
-
-Notation MIEnvFilter C := (MIEnvTransform (TCDiag C)).
-
-Definition modality_intro_spec_persistent {PROP1 PROP2}
-    (s : modality_intro_spec PROP1 PROP2) : (PROP1 → PROP2) → Prop :=
-  match s with
-  | MIEnvIsEmpty => λ M, True
-  | MIEnvForall C => λ M,
-     (∀ P, C P → □ P ⊢ M (□ P)) ∧
-     (∀ P Q, M P ∧ M Q ⊢ M (P ∧ Q))
-  | MIEnvTransform C => λ M,
-     (∀ P Q, C P Q → □ P ⊢ M (□ Q)) ∧
-     (∀ P Q, M P ∧ M Q ⊢ M (P ∧ Q))
-  | MIEnvClear => λ M, True
-  | MIEnvId => λ M, ∀ P, □ P ⊢ M (□ P)
-  end.
-
-Definition modality_intro_spec_spatial {PROP1 PROP2}
-    (s : modality_intro_spec PROP1 PROP2) : (PROP1 → PROP2) → Prop :=
-  match s with
-  | MIEnvIsEmpty => λ M, True
-  | MIEnvForall C => λ M, ∀ P, C P → P ⊢ M P
-  | MIEnvTransform C => λ M, ∀ P Q, C P Q → P ⊢ M Q
-  | MIEnvClear => λ M, ∀ P, Absorbing (M P)
-  | MIEnvId => λ M, ∀ P, P ⊢ M P
-  end.
-
-(* A modality is then a record packing together the modality with the laws it
-should satisfy to justify the given actions for both contexts: *)
-Record modality_mixin {PROP1 PROP2 : bi} (M : PROP1 → PROP2)
-    (pspec sspec : modality_intro_spec PROP1 PROP2) := {
-  modality_mixin_persistent : modality_intro_spec_persistent pspec M;
-  modality_mixin_spatial : modality_intro_spec_spatial sspec M;
-  modality_mixin_emp : emp ⊢ M emp;
-  modality_mixin_mono P Q : (P ⊢ Q) → M P ⊢ M Q;
-  modality_mixin_sep P Q : M P ∗ M Q ⊢ M (P ∗ Q)
-}.
-
-Record modality (PROP1 PROP2 : bi) := Modality {
-  modality_car :> PROP1 → PROP2;
-  modality_persistent_spec : modality_intro_spec PROP1 PROP2;
-  modality_spatial_spec : modality_intro_spec PROP1 PROP2;
-  modality_mixin_of :
-    modality_mixin modality_car modality_persistent_spec modality_spatial_spec
-}.
-Arguments Modality {_ _} _ {_ _} _.
-Arguments modality_persistent_spec {_ _} _.
-Arguments modality_spatial_spec {_ _} _.
-
-Section modality.
-  Context {PROP1 PROP2} (M : modality PROP1 PROP2).
-
-  Lemma modality_persistent_transform C P Q :
-    modality_persistent_spec M = MIEnvTransform C → C P Q → □ P ⊢ M (□ Q).
-  Proof. destruct M as [??? []]; naive_solver. Qed.
-  Lemma modality_and_transform C P Q :
-    modality_persistent_spec M = MIEnvTransform C → M P ∧ M Q ⊢ M (P ∧ Q).
-  Proof. destruct M as [??? []]; naive_solver. Qed.
-  Lemma modality_spatial_transform C P Q :
-    modality_spatial_spec M = MIEnvTransform C → C P Q → P ⊢ M Q.
-  Proof. destruct M as [??? []]; naive_solver. Qed.
-  Lemma modality_spatial_clear P :
-    modality_spatial_spec M = MIEnvClear → Absorbing (M P).
-  Proof. destruct M as [??? []]; naive_solver. Qed.
-
-  Lemma modality_emp : emp ⊢ M emp.
-  Proof. eapply modality_mixin_emp, modality_mixin_of. Qed.
-  Lemma modality_mono P Q : (P ⊢ Q) → M P ⊢ M Q.
-  Proof. eapply modality_mixin_mono, modality_mixin_of. Qed.
-  Lemma modality_sep P Q : M P ∗ M Q ⊢ M (P ∗ Q).
-  Proof. eapply modality_mixin_sep, modality_mixin_of. Qed.
-  Global Instance modality_mono' : Proper ((⊢) ==> (⊢)) M.
-  Proof. intros P Q. apply modality_mono. Qed.
-  Global Instance modality_flip_mono' : Proper (flip (⊢) ==> flip (⊢)) M.
-  Proof. intros P Q. apply modality_mono. Qed.
-  Global Instance modality_proper : Proper ((≡) ==> (≡)) M.
-  Proof. intros P Q. rewrite !equiv_spec=> -[??]; eauto using modality_mono. Qed.
-End modality.
-
-Section modality1.
-  Context {PROP} (M : modality PROP PROP).
-
-  Lemma modality_persistent_forall C P :
-    modality_persistent_spec M = MIEnvForall C → C P → □ P ⊢ M (□ P).
-  Proof. destruct M as [??? []]; naive_solver. Qed.
-  Lemma modality_and_forall C P Q :
-    modality_persistent_spec M = MIEnvForall C → M P ∧ M Q ⊢ M (P ∧ Q).
-  Proof. destruct M as [??? []]; naive_solver. Qed.
-  Lemma modality_persistent_id P :
-    modality_persistent_spec M = MIEnvId → □ P ⊢ M (□ P).
-  Proof. destruct M as [??? []]; naive_solver. Qed.
-  Lemma modality_spatial_forall C P :
-    modality_spatial_spec M = MIEnvForall C → C P → P ⊢ M P.
-  Proof. destruct M as [??? []]; naive_solver. Qed.
-  Lemma modality_spatial_id P :
-    modality_spatial_spec M = MIEnvId → P ⊢ M P.
-  Proof. destruct M as [??? []]; naive_solver. Qed.
-
-  Lemma modality_persistent_forall_big_and C Ps :
-    modality_persistent_spec M = MIEnvForall C →
-    Forall C Ps → □ [∧] Ps ⊢ M (□ [∧] Ps).
-  Proof.
-    induction 2 as [|P Ps ? _ IH]; simpl.
-    - by rewrite persistently_pure affinely_True_emp affinely_emp -modality_emp.
-    - rewrite affinely_persistently_and -modality_and_forall // -IH.
-      by rewrite {1}(modality_persistent_forall _ P).
-  Qed.
-  Lemma modality_spatial_forall_big_sep C Ps :
-    modality_spatial_spec M = MIEnvForall C →
-    Forall C Ps → [∗] Ps ⊢ M ([∗] Ps).
-  Proof.
-    induction 2 as [|P Ps ? _ IH]; simpl.
-    - by rewrite -modality_emp.
-    - by rewrite -modality_sep -IH {1}(modality_spatial_forall _ P).
-  Qed.
-End modality1.
-
 (** The [FromModal M P Q] class is used by the [iModIntro] tactic to transform
 a goal [P] into a modality [M] and proposition [Q].
 
-The input is [P] and the outputs are [M] and [Q]. *)
+The input is [P] and the outputs are [M] and [Q].
+
+For modalities [M] that do not need to augment the proof mode environment, one
+can define an instance [FromModal modality_id (M P) P]. Defining such an
+only imposes the proof obligation [P ⊢ M P]. Examples of modalities that have
+such an instance are [bupd], [fupd], [except_0], [monPred_relatively] and
+[bi_absorbingly]. *)
 Class FromModal {PROP1 PROP2 : bi}
     (M : modality PROP1 PROP2) (P : PROP2) (Q : PROP1) :=
   from_modal : M Q ⊢ P.
 Arguments FromModal {_ _} _ _%I _%I : simpl never.
 Arguments from_modal {_ _} _ _%I _%I {_}.
 Hint Mode FromModal - + - ! - : typeclass_instances.
-
-(** The identity modality [modality_id] can be used in combination with
-[FromModal modality_id] to support introduction for modalities that enjoy
-[P ⊢ M P]. This is done by defining an instance [FromModal modality_id (M P) P],
-which will instruct [iModIntro] to introduce the modality without modifying the
-proof mode context. Examples of such modalities are [bupd], [fupd], [except_0],
-[monPred_relatively] and [bi_absorbingly]. *)
-Lemma modality_id_mixin {PROP : bi} : modality_mixin (@id PROP) MIEnvId MIEnvId.
-Proof. split; simpl; eauto. Qed.
-Definition modality_id {PROP : bi} := Modality (@id PROP) modality_id_mixin.
 
 Class FromAffinely {PROP : bi} (P Q : PROP) :=
   from_affinely : bi_affinely Q ⊢ P.
