theories/proofmode/class_instances.v
@@ -1,6 +1,6 @@
 From stdpp Require Import nat_cancel.
 From iris.bi Require Import bi tactics.
-From iris.proofmode Require Export classes.
+From iris.proofmode Require Export modality_instances classes.
 Set Default Proof Using "Type".
 Import bi.
 
